foterms_std.v
@@ -1,0 +1,33 @@
+(* First-Order Terms with no eigen variables *)
+
+Require Import stdlib_more.
+Require Export foterms.
+
+Set Implicit Arguments.
+
+
+Section Terms.
+
+Context { vatom : DecType } { tatom fatom : Type }.
+
+Notation "r ;; s" := (fecomp r s) (at level 20, format "r  ;;  s").
+Notation closed t := (tvars t = nil).
+Notation fclosed r := (forall n, closed (r n)).
+
+Arguments tvar {_} {_} {T} _.
+
+(* Function allowing to embed [term Empty_set] into any [term T]
+     through identity embedding by using [tesubs (r_empty T)] *)
+Definition r_empty T : Empty_set -> @term vatom tatom T := fun z =>
+  match z with end.
+
+Lemma fclosed_r_empty T : fclosed (r_empty T).
+Proof. intros n; destruct n. Qed.
+Hint Resolve fclosed_r_empty : term_db.
+
+Lemma fecomp_r_empty T1 T2 : forall s, r_empty T1 ;; s == r_empty T2.
+Proof. intros s n; destruct n. Qed.
+Hint Rewrite fecomp_r_empty : term_db.
+
+End Terms.
+
