hilbert2nj.v
@@ -1,7 +1,9 @@
 (* From Hilbert System to Natural Deduction *)
 
 Require Import stdlib_more.
-Require Export nj1 hilbert.
+Require Export foterms_std nj1 hilbert.
+
+Set Implicit Arguments.
 
 
 Section H2N.
@@ -15,6 +17,7 @@ Notation hformula := (@formula vatom tatom fatom Nocon Icon Qcon Empty_set).
 
 Notation term := (@term vatom tatom nat).
 Notation formula := (@formula vatom tatom fatom Nocon Icon Qcon nat).
+Notation r_h2n := (@r_empty vatom tatom nat).
 Notation closed t := (tvars t = nil).
 Notation fclosed r := (forall n, closed (r n)).
 Notation "↑ r" := (felift r) (at level 25, format "↑ r").
@@ -26,9 +29,21 @@ Notation "L ∖ x" := (remove_snd x L) (at level 18).
 Notation "⇑" := fup.
 Notation "A ↑" := (A⟦⇑⟧) (at level 8, format "A ↑").
 Notation "x ∈ A" := (In x (freevars A)) (at level 30).
+Notation "x ∉ A" := (~ In x (freevars A)) (at level 30).
 Notation "y #[ x ] A" := (no_capture_at x y A) (at level 30, format "y  #[ x ]  A").
 
 Infix "→" := (fbin imp_con) (at level 55, right associativity).
+
+Hint Rewrite (@tsubs_tesubs vatom tatom Empty_set nat)
+                          using try (intuition; fail);
+                               (try apply fclosed_no_tecapture); intuition; fail : term_db.
+
+Hint Resolve (@fclosed_r_empty vatom tatom) : term_db.
+Hint Rewrite (@fecomp_r_empty vatom tatom) : term_db.
+
+Hint Resolve (@fclosed_no_tecapture vatom tatom Empty_set nat) : term_db.
+Hint Resolve (@fclosed_no_ecapture vatom tatom fatom Nocon Icon Qcon Empty_set nat) : term_db.
+Hint Resolve (@no_ecapture_not_egenerated vatom tatom fatom Nocon Icon Qcon Empty_set nat) : term_db.
 
 Ltac run_ax :=
   match goal with
@@ -37,55 +52,10 @@ Ltac run_ax :=
   end.
 Ltac auto_ax := rewrite <- (app_nil_l _); run_ax.
 
-(* Translation of terms: trivial embedding *)
-Fixpoint h2n_term (t : hterm) : term :=
-match t with
-| tvar x => tvar x
-| dvar z => match z with end
-| tconstr f l => tconstr f (map h2n_term l)
-end.
 
-Lemma h2n_tvars : forall t, tvars (h2n_term t) = tvars t.
-Proof. term_induction t. Qed.
-
-Lemma h2n_closed : forall t, closed t <-> closed (h2n_term t).
-Proof. intros t; rewrite h2n_tvars; intuition. Qed.
-
-Lemma h2n_tsubs : forall x u t,
-  h2n_term (tsubs x u t) = tsubs x (h2n_term u) (h2n_term t).
-Proof. term_induction t. Qed.
-Hint Rewrite h2n_tsubs : term_db.
-
-Lemma h2n_tesubs : forall r t, tesubs r (h2n_term t) = h2n_term t.
-Proof. term_induction t. Qed.
-Hint Rewrite h2n_tesubs : term_db.
-
-(* Translation of formulas: trivial embedding *)
-Fixpoint h2n_formula (A : hformula) : formula :=
-match A with
-| fvar X l => fvar X (map h2n_term l)
-| fnul _ ncon => match ncon with end
-| fbin bcon B C => fbin bcon (h2n_formula B) (h2n_formula C)
-| fqtf qcon y B => fqtf qcon y (h2n_formula B)
-end.
-
-Lemma h2n_freevars : forall A, freevars (h2n_formula A) = freevars A.
-Proof. formula_induction A; (try now rewrite ? IHA1, ? IHA2, ? IHA); apply h2n_tvars. Qed.
-
-Lemma h2n_closed_formula : forall A, freevars A = nil <-> freevars (h2n_formula A) = nil.
-Proof. intros A; rewrite h2n_freevars; intuition. Qed.
-
-Lemma h2n_subs : forall x u A,
-  h2n_formula (A[u//x]) = (h2n_formula A)[h2n_term u//x].
-Proof. formula_induction A. Qed.
-Hint Rewrite h2n_subs : term_db.
-
-Lemma h2n_esubs : forall r A, (h2n_formula A)⟦r⟧ = h2n_formula A.
-Proof. formula_induction A. Qed.
-Hint Rewrite h2n_esubs : term_db.
-
-Lemma h2n_no_capture : forall x y A, y #[x] A -> y #[x] (h2n_formula A).
-Proof. formula_induction A; rewrite h2n_freevars in H0; intuition. Qed.
+(* Translation of terms and formulas: trivial embedding *)
+Notation h2n_term := (@tesubs vatom tatom Empty_set nat r_h2n).
+Notation h2n_formula := (@esubs vatom tatom fatom Nocon Icon Qcon Empty_set nat r_h2n).
 
 Proposition h2n : forall A, hprove A ->
   forall L, Forall (fun z => closed z) (map snd L) -> incl (freevars A) (map fst L) ->
@@ -117,25 +87,26 @@ intros A pi; induction pi; intros L Hcl Hsub;
   apply (impe AAA).
   + specialize IHpi1 with (L ++ LA).
     simpl in IHpi1; rewrite ? multi_subs_fbin in IHpi1.
-    subst AAA BB; rewrite multi_subs_ext with (L':= LA) (A0:= h2n_formula B);
-      [ apply IHpi1 | assumption | rewrite h2n_freevars ]; rewrite ? map_app; intuition.
+    subst AAA BB; rewrite multi_subs_extend with (L':= LA) (A0:= h2n_formula B);
+      [ apply IHpi1 | assumption | rewrite freevars_esubs_fclosed ]; rewrite ? map_app; intuition.
     * apply Forall_app; intuition.
     * apply incl_app; [ apply incl_appr | apply incl_appl ]; intuition.
       rewrite HfstLA; apply incl_refl.
   + subst AAA; apply IHpi2; rewrite ? map_app.
     * apply Forall_app; intuition.
     * apply incl_appr; rewrite HfstLA; apply incl_refl.
-- rewrite multi_subs_fqtf, h2n_subs, multi_subs_subs; intuition.
+- rewrite multi_subs_fqtf, subs_esubs, multi_subs_subs; intuition.
   + destruct (in_dec eq_dt_dec x (freevars (h2n_formula A))) as [Hf|Hf].
     * apply frle; [ | apply ax_hd ].
       clear - f Hcl Hsub Hf.
       apply multi_tsubs_closed; [ assumption | ].
       intros z Hinz.
       apply Hsub; simpl.
-      rewrite h2n_freevars in Hf; rewrite h2n_tvars in Hinz.
+      rewrite freevars_esubs_fclosed in Hf; [ | intuition ].
+      rewrite tvars_tesubs_fclosed in Hinz; [ | intuition ].
       apply no_capture_subs_freevars with (x0:= z) (u:= t) in Hf; intuition.
       now specialize_Forall f with z.
-    * assert (~ x ∈ (h2n_formula A)[[L ∖ x]]) as Hnin.
+    * assert (x ∉ (h2n_formula A)[[L ∖ x]]) as Hnin.
       { intros Hin; apply Hf; apply multi_subs_freevars in Hin; try assumption.
         apply Forall_incl with (map snd L); intuition.
         clear; induction L; intuition; simpl; case_analysis; intuition. }
@@ -145,9 +116,9 @@ intros A pi; induction pi; intros L Hcl Hsub;
       rewrite nfree_subs by assumption.
       apply ax_hd.
   + apply Forall_forall; intros z Hinz.
-    rewrite h2n_tvars in Hinz.
+    rewrite tvars_tesubs_fclosed in Hinz; [ | intuition ].
     specialize_Forall f with z.
-    now apply h2n_no_capture.
+    apply no_capture_esubs; intuition.
 - rewrite ? multi_subs_fqtf.
   rewrite <- @multi_subs_remove with (x:=x) in HeqAA; try assumption.
   + apply frli; simpl.
@@ -160,13 +131,13 @@ intros A pi; induction pi; intros L Hcl Hsub;
     intros Hin; apply n.
     rewrite freevars_fup in Hin; subst.
     apply multi_subs_freevars in Hin.
-    * now rewrite <- h2n_freevars.
+    * now rewrite <- freevars_esubs_fclosed with (r:= r_h2n).
     * apply Forall_incl with (map snd L); intuition.
       clear; induction L; intuition; simpl; case_analysis; intuition.
-  + now rewrite h2n_freevars.
+  + now rewrite freevars_esubs_fclosed.
 - rewrite multi_subs_fqtf.
   apply frli; simpl.
-  rewrite multi_subs_esubs, h2n_esubs by (apply Forall_forall; intuition).
+  rewrite multi_subs_esubs, esubs_comp, esubs_ext with (r2:=r_h2n); intuition.
   replace (((h2n_formula A)[[map (fun '(x0, u) => (x0, tesubs ⇑ u)) (L ∖ x)]])[dvar 0//x])
      with (((h2n_formula A)[[map (fun '(x0, u) => (x0, tesubs ⇑ u)) (L ∖ x)
                              ++ (x, dvar 0) :: nil]]))
@@ -187,17 +158,19 @@ intros A pi; induction pi; intros L Hcl Hsub;
     rewrite <- remove_snd_remove.
     eapply notin_remove with (y:= x) in Hinz; intuition ; apply Hsub in Hinz.
     apply notin_remove with (Hdec:= eq_dt_dec) (y:= x) in Hinz; intuition.
-- rewrite multi_subs_fqtf, h2n_subs, multi_subs_subs; try assumption.
+- rewrite multi_subs_fqtf, subs_esubs; intuition.
+  rewrite multi_subs_subs; try assumption.
   + destruct (in_dec eq_dt_dec x (freevars (h2n_formula A))) as [Hf|Hf].
     * eapply exsi; [ | apply ax_hd ].
       clear - f Hcl Hsub Hf.
       apply multi_tsubs_closed; [ assumption | ].
       intros z Hinz.
       apply Hsub; simpl.
-      rewrite h2n_freevars in Hf; rewrite h2n_tvars in Hinz.
+      rewrite freevars_esubs_fclosed in Hf; intuition.
+      rewrite tvars_tesubs_fclosed in Hinz; intuition.
       apply no_capture_subs_freevars with (x0:= z) (u:= t) in Hf; intuition.
       now specialize_Forall f with z.
-    * assert (~ x ∈ (h2n_formula A)[[L ∖ x]]) as Hnin.
+    * assert (x ∉ (h2n_formula A)[[L ∖ x]]) as Hnin.
       { intros Hin; apply Hf; apply multi_subs_freevars in Hin; try assumption.
         apply Forall_incl with (map snd L); intuition.
         clear; induction L; intuition; simpl; case_analysis; intuition. }
@@ -206,9 +179,9 @@ intros A pi; induction pi; intros L Hcl Hsub;
       rewrite nfree_subs by assumption.
       apply ax_hd.
   + apply Forall_forall; intros z Hinz.
-    rewrite h2n_tvars in Hinz.
+    rewrite tvars_tesubs_fclosed in Hinz; [ | intuition ].
     specialize_Forall f with z.
-    now apply h2n_no_capture.
+    now apply no_capture_esubs.
 - rewrite 2 multi_subs_fqtf.
   rewrite <- @multi_subs_remove with (x:=x) in HeqBB; try assumption.
   + apply @exse with (x:=x) (A:= (h2n_formula A)[[L ∖ x]]); [ apply ax_hd | ].
@@ -220,10 +193,10 @@ intros A pi; induction pi; intros L Hcl Hsub;
     intros Hin; apply n.
     rewrite freevars_fup in Hin; subst.
     apply multi_subs_freevars in Hin.
-    * now rewrite <- h2n_freevars.
+    * now rewrite <- freevars_esubs_fclosed with (r:=r_h2n).
     * apply Forall_incl with (map snd L); intuition.
       clear; induction L; intuition; simpl; case_analysis; intuition.
-  + now rewrite h2n_freevars.
+  + now rewrite freevars_esubs_fclosed.
 Qed.
 
 End H2N.
